coq/v2/Properties/IPR_old.v
@@ -1,0 +1,1011 @@
+Require Import Koika.Frontend.
+Require Import Koika.Std.
+Require Import Koika.Utils.Common.
+Require Import Koika.Utils.Environments.
+Require Koika.Properties.SemanticProperties.
+Require Koika.KoikaForm.Untyped.UntypedSemantics.
+Require Import Koika.KoikaForm.SimpleVal.
+
+Require Import Trustformer.v2.Syntax.
+Require Import Trustformer.v2.Semantics.
+Require Import Trustformer.v2.Synthesis.
+Require Import Trustformer.v2.Utils.
+Require Trustformer.v2.Properties.Common.
+From Koika.Utils Require Import Tactics.
+
+Require Import Coq.Logic.FunctionalExtensionality.
+
+Require Import Streams.
+Require Import Coq.Lists.List.
+Require Import Coq.Strings.String.
+Require Import Coq.Logic.Eqdep_dec.
+Require Import Coq.Init.Tactics.
+
+Require Import Hammer.Plugin.Hammer.
+Set Hammer GSMode 63.
+
+
+Section CompositionalCorrectness.
+
+    (* Generalize over any input to the synthesis *)
+    Context (some_fs_states: Type).
+    Context (some_fs_states_fin : FiniteType some_fs_states).
+    Context (some_fs_states_names : Show some_fs_states).
+    Context (some_fs_states_size : some_fs_states -> nat).
+    Context (some_fs_states_init : forall x: some_fs_states, tf_states_type some_fs_states some_fs_states_size x).
+
+    Context (some_fs_inputs : Type).
+    Context (some_fs_inputs_fin : FiniteType some_fs_inputs).
+    Context (some_fs_inputs_names : Show some_fs_inputs).
+    Context (some_fs_inputs_size : some_fs_inputs -> nat).
+
+    Context (some_fs_outputs : Type).
+    Context (some_fs_outputs_fin : FiniteType some_fs_outputs).
+    Context (some_fs_outputs_names : Show some_fs_outputs).
+    Context (some_fs_outputs_size : some_fs_outputs -> nat).
+
+    Context (some_fs_action : Type).
+    Context (some_fs_action_fin : FiniteType some_fs_action).
+    Context (some_fs_action_names : Show some_fs_action).
+    Context (some_fs_action_ops : some_fs_action -> tf_ops some_fs_states some_fs_inputs some_fs_outputs).
+
+    (* We craft the tx_context here as it leads to cleaner proofs than generalizing over it*)
+    Definition tf_ctx := {|
+      tf_spec_states := some_fs_states;
+      tf_spec_states_fin := some_fs_states_fin;
+      tf_spec_states_names := some_fs_states_names;
+      tf_spec_states_size := some_fs_states_size;
+      tf_spec_states_init := some_fs_states_init;
+
+      tf_spec_inputs := some_fs_inputs;
+      tf_spec_inputs_fin := some_fs_inputs_fin;
+      tf_spec_inputs_names := some_fs_inputs_names;
+      tf_spec_inputs_size := some_fs_inputs_size;
+
+      tf_spec_outputs := some_fs_outputs;
+      tf_spec_outputs_fin := some_fs_outputs_fin;
+      tf_spec_outputs_names := some_fs_outputs_names;
+      tf_spec_outputs_size := some_fs_outputs_size;
+
+      tf_spec_action := some_fs_action;
+      tf_spec_action_fin := some_fs_action_fin;
+      tf_spec_action_names := some_fs_action_names;
+      tf_spec_action_ops := some_fs_action_ops
+    |}.
+    Definition some_fs_states_t := tf_states_type some_fs_states some_fs_states_size.
+
+    Context (sigma: (ext_fn_t tf_ctx) -> val -> val).
+    Context (sigma_valid: 
+     forall f x, 
+     exists (f_t : retSig (Sigma tf_ctx f)),
+     sigma f x = val_of_value f_t
+    ).
+
+    (* Obtain the various outputs of the synthesis *)
+    Definition some_R := R tf_ctx.
+    Definition some_r := r tf_ctx.
+    Definition some_rules := rules tf_ctx.
+    Definition some_system_schedule := system_schedule tf_ctx.
+    Definition some_reg_t := reg_t tf_ctx.
+    Definition some_cmd_reg_size := cmd_reg_size tf_ctx.
+
+    Instance some_reg_t_finite : FiniteType (some_reg_t) := _reg_t_finite tf_ctx.
+    Definition some_reg_t_elements := @finite_elements some_reg_t some_reg_t_finite.
+    Definition some_fs_state_elements := @finite_elements some_fs_states some_fs_states_fin.
+
+
+    (* Encoding of commands as bitvectors *)
+    Definition _fs_cmd_encoding (a: some_fs_action) :=
+      Bits.of_nat some_cmd_reg_size (@finite_index some_fs_action _ a).
+    Definition _encoded_cmd (a: some_fs_action) : type_denote (maybe (bits_t some_cmd_reg_size)) :=
+        (Ob~1, (_fs_cmd_encoding a, tt)).
+    Definition encoded_cmd (a: some_fs_action) := val_of_value (_encoded_cmd a).
+
+    Definition val_true := Bits ( [true] ).
+
+  (* Properties about the encoding of commands *)
+  Section Encoding.
+
+    Example val_of_value_for_cmd_is_struct :
+    forall (a : some_fs_action),
+      let sig := Maybe (bits_t some_cmd_reg_size) in
+      encoded_cmd a
+      =
+      Struct sig [val_true; Bits (vect_to_list (_fs_cmd_encoding a))].
+    Proof.
+      intros. unfold encoded_cmd, _encoded_cmd. reflexivity.
+    Qed.
+
+    Lemma encoded_cmd_inj :
+      forall (a1 a2 : some_fs_action),
+      encoded_cmd a1 = encoded_cmd a2 -> a1 = a2.
+    Proof.
+      intros a1 a2 H_eq.
+      unfold encoded_cmd, _encoded_cmd in H_eq.
+      unfold _fs_cmd_encoding in H_eq.
+      timeout 10 simpl in H_eq.
+      apply f_equal with (f:=ubits_of_value) in H_eq.
+      timeout 10 cbn -[vect_to_list] in H_eq.
+      apply app_inj_tail in H_eq.
+      destruct H_eq as [H_bits_eq H_ob_eq]. clear H_ob_eq.
+      apply vect_to_list_inj in H_bits_eq.
+      apply f_equal with (f:=Bits.to_nat) in H_bits_eq.
+      rewrite Bits.to_nat_of_nat in H_bits_eq.
+      rewrite Bits.to_nat_of_nat in H_bits_eq.
+      - apply finite_index_injective. exact H_bits_eq.
+      - rewrite pow2_correct. unfold some_cmd_reg_size, cmd_reg_size. apply Common.finite_bits_needed_correct.
+      - rewrite pow2_correct. unfold some_cmd_reg_size, cmd_reg_size. apply Common.finite_bits_needed_correct.
+    Qed.
+
+    Lemma encoded_cmd_inj' :
+      forall (a1 a2 : some_fs_action),
+      a1 <> a2 ->
+      encoded_cmd a1 <> encoded_cmd a2.
+    Proof.
+      intros a1 a2 H_neq. intros H_eq.
+      apply encoded_cmd_inj in H_eq.
+      contradiction.
+    Qed.    
+
+    Lemma sigma_ext_in_cmd_is_struct :
+      forall (cmd : some_fs_action) vars,
+      exists valid' cmd_encoding,
+      sigma (ext_in_cmd tf_ctx) vars = Struct (Maybe (bits_t some_cmd_reg_size)) [Bits [valid']; Bits cmd_encoding].
+    Proof.
+      intros.
+      specialize (sigma_valid (ext_in_cmd tf_ctx) vars).
+      unfold retSig, Sigma, val_of_value, some_cmd_reg_size in *.
+      destruct sigma_valid as [f_t Heq].
+      destruct f_t as [b v_and_unit].
+      destruct v_and_unit as [v H_unit].
+      rewrite Heq.
+      eexists _,_.
+      simpl.
+      reflexivity.
+    Qed.   
+
+    Lemma cmd_rule_eq_dec_equal:
+      forall (cmd1 cmd2: some_fs_action),
+        (rule_cmd tf_ctx cmd1) = (rule_cmd tf_ctx cmd2) <-> cmd1 = cmd2.
+    Proof.
+        intros. split.
+        - intros H_eq. inversion H_eq. reflexivity.
+        - intros H_eq. rewrite H_eq. reflexivity.
+    Qed.
+
+    Lemma cmd_rule_eq_dec_if:
+      forall (cmd1 cmd2: some_fs_action) a b,
+        (if eq_dec (rule_cmd tf_ctx cmd1) (rule_cmd tf_ctx cmd2)
+        then a
+        else b) ->
+        ((cmd1 = cmd2 -> a) /\ (cmd1 <> cmd2 -> b)).
+    Proof.
+        intros. destruct (eq_dec (rule_cmd tf_ctx cmd1) (rule_cmd tf_ctx cmd2)) as [H_eq | H_neq].
+        - assert (cmd1 = cmd2) as H_cmd_eq.
+          { apply cmd_rule_eq_dec_equal. exact H_eq. }
+          timeout 10 sauto.
+        - timeout 10 sauto.
+    Qed.
+
+    Lemma reg_name_injective :
+      forall r1 r2,
+        (_reg_name tf_ctx r1) = (_reg_name tf_ctx r2) -> r1 = r2.
+    Proof.
+      intros. unfold _reg_name in H.
+      timeout 10 simpl in H. unfold spec_state_index in H.
+      injection H. intros.
+      apply finite_index_injective.
+      apply string_id_of_nat_inj in H0.
+      timeout 10 sauto.
+    Qed.
+
+  End Encoding. 
+
+    (* Other helpful definitions *)
+  Definition hw_env_t := env_t ContextEnv (fun _ : some_reg_t => val).
+
+  Section CmdGuard.
+    
+    Lemma interp_rule_wrong_cmd:
+      forall (hw_reg_state: hw_env_t) log cmd,
+      sigma (ext_in_cmd tf_ctx) val_true <> encoded_cmd cmd ->
+      UntypedSemantics.interp_rule hw_reg_state sigma log (some_rules (rule_cmd tf_ctx cmd)) = None.
+    Proof.
+      intros.
+      unfold some_rules, rules, _rule_cmd.
+      unfold UntypedSemantics.interp_rule, UntypedSemantics.interp_action.
+
+      cbn. unfold val_true.
+
+      (* We know what in_cmd will give as a result so lets substitute it in our code *)
+      set (sigma_val := sigma (ext_in_cmd tf_ctx) (Bits [true])) in *.
+      assert (HSigmaValCmd: sigma_val <> encoded_cmd cmd).
+      { unfold sigma_val. exact H. }
+      destruct sigma_val eqn:H_sigma_val.
+      cbn. timeout 10 sauto. cbn. timeout 10 sauto.
+      { remember (BitsToLists.get_field (Struct sig v) "valid") as valid_field_opt.
+        destruct valid_field_opt eqn:H_cmd_valid.
+        { cbn. destruct v0.
+          { cbn. destruct v0.
+            cbn. timeout 10 sauto. cbn. destruct v0.
+            { cbn. destruct b.
+              {
+                cbn. remember (BitsToLists.get_field_struct (struct_fields sig) v "data") as data_field_opt.
+                destruct data_field_opt.
+                { cbn. destruct v0.
+                  { cbn. 
+                    assert (BitsToLists.list_eqb Bool.eqb v0 (vect_to_list (Bits.of_nat (cmd_reg_size tf_ctx) (spec_action_index tf_ctx cmd))) = false).
+                    { 
+                      rewrite <- Bool.not_true_iff_false.
+                      rewrite BitsToLists.list_eqb_correct.
+                      {
+                        intro H_eq. subst v0. subst sigma_val. clear valid_field_opt H_cmd_valid.
+                        timeout 10 cbn in *. unfold not in *.
+                        unfold _fs_cmd_encoding, some_cmd_reg_size, spec_action_index, spec_action, spec_action_fin in *.
+                        unfold tf_ctx, tf_spec_action, tf_spec_action_fin in *. fold tf_ctx in *.
+                        apply HSigmaValCmd.
+                        generalize (sigma_ext_in_cmd_is_struct cmd (Bits [true])); intros.
+                        rewrite H_sigma_val in *. 
+
+                        destruct H0 as [valid' [cmd_encoding H_sigma_struct]].
+                        f_equal. timeout 10 sauto.
+                        injection H_sigma_struct as Heqv.
+                        rewrite Heqv in *. clear Heqv. rewrite H0 in *. clear H0.
+
+                        unfold BitsToLists.get_field_struct in *.
+                        f_equal. f_equal.
+                        { timeout 10 sauto. }
+                        { timeout 10 sauto. }
+                    
+                      } intros. split. intros. destruct a, b. timeout 10 sauto. timeout 10 sauto. timeout 10 sauto. timeout 10 sauto. 
+                        intros. rewrite H0. destruct b. timeout 10 sauto. timeout 10 sauto.
+                    } rewrite H0. cbn. timeout 10 sauto.
+                  } cbn. timeout 10 sauto. cbn. timeout 10 sauto. cbn. timeout 10 sauto.
+                } cbn. timeout 10 sauto.
+              } cbn. timeout 10 sauto.                         
+            } cbn. timeout 10 sauto.
+          } cbn. timeout 10 sauto. cbn. timeout 10 sauto. cbn. timeout 10 sauto.            
+        } cbn. timeout 10 sauto.  
+       } cbn. timeout 10 sauto.
+    Qed.
+
+    Lemma interp_scheduler_no_cmd:
+      forall (hw_reg_state: hw_env_t) cmd schedule log,
+      sigma (ext_in_cmd tf_ctx) val_true = encoded_cmd cmd ->
+      (~ Common.scheduler_has_rule schedule (rule_cmd tf_ctx cmd)) ->
+      UntypedSemantics.interp_scheduler' some_rules hw_reg_state sigma log schedule = log.
+    Proof.
+      intros. unfold UntypedSemantics.interp_scheduler, UntypedSemantics.interp_scheduler'.
+
+      induction schedule. reflexivity.
+      {
+        rewrite IHschedule. clear IHschedule.
+        {
+          unfold not, Common.scheduler_has_rule in H0.
+          destruct r. destruct (eq_dec cmd0 cmd).
+          - subst cmd0. destruct (eq_dec (rule_cmd tf_ctx cmd) (rule_cmd tf_ctx cmd)).
+            + exfalso. apply H0. sauto.
+            + exfalso. unfold not in n. generalize (cmd_rule_eq_dec_equal cmd cmd). intros. inversion H1. timeout 10 sauto.
+          - rewrite interp_rule_wrong_cmd.
+            + timeout 10 sauto.
+            + generalize (encoded_cmd_inj' cmd0 cmd). intros. timeout 10 sauto.
+        }
+        {
+          generalize (Common.scheduler_has_not_rule_inductive (r |> schedule) (rule_cmd tf_ctx cmd) ).
+          intros.
+          pose proof (H1 H0) as H_derived.
+          destruct (eq_dec r (rule_cmd tf_ctx cmd)) as [H_eq | H_neq].
+          - exfalso. contradiction.
+          - exact H_derived.
+        }
+      }
+      {
+        rewrite IHschedule2. clear IHschedule2.
+        {
+          unfold not, Common.scheduler_has_rule in H0.
+          destruct r. destruct (eq_dec cmd0 cmd).
+          - subst cmd0. destruct (eq_dec (rule_cmd tf_ctx cmd) (rule_cmd tf_ctx cmd)).
+            + exfalso. apply H0. sauto.
+            + exfalso. unfold not in n. generalize (cmd_rule_eq_dec_equal cmd cmd). intros. inversion H1. timeout 10 sauto.
+          - rewrite interp_rule_wrong_cmd.
+            + timeout 10 sauto.
+            + generalize (encoded_cmd_inj' cmd0 cmd). intros. timeout 10 sauto.
+
+        }
+        {
+          generalize (Common.scheduler_has_not_rule_inductive (Try r schedule1 schedule2) (rule_cmd tf_ctx cmd) ).
+          intros.
+          pose proof (H1 H0) as H_derived.
+          destruct (eq_dec r (rule_cmd tf_ctx cmd)) as [H_eq | H_neq].
+          - exfalso. contradiction.
+          - timeout 10 sauto.
+        }
+      }
+      {
+        rewrite IHschedule. clear IHschedule.
+        timeout 10 sauto.
+        {
+          generalize (Common.scheduler_has_not_rule_inductive (SPos p schedule) (rule_cmd tf_ctx cmd) ).
+          intros.
+          pose proof (H1 H0) as H_derived.
+          timeout 10 sauto.
+        }
+      }
+    Qed.
+
+    Lemma interp_scheduler_only_cmd:
+      forall (hw_reg_state: hw_env_t) cmd,
+      sigma (ext_in_cmd tf_ctx) val_true = encoded_cmd cmd ->
+      UntypedSemantics.interp_scheduler some_rules hw_reg_state sigma some_system_schedule = 
+      UntypedSemantics.interp_scheduler some_rules hw_reg_state sigma ( rule_cmd tf_ctx cmd |> done ).
+    Proof.
+      intros.
+      unfold UntypedSemantics.interp_scheduler.
+      (* unfold UntypedSemantics.interp_scheduler'. *)
+
+      set (schedule := some_system_schedule) in *.
+      unfold some_system_schedule, system_schedule, system_schedule_actions in *.
+      unfold spec_all_actions in *.
+
+      set (action_order := finite_elements) in *.
+
+      assert (NoDup (action_order)).
+      {
+        apply NoDup_map_inv with (f:=finite_index).
+        apply finite_injective.
+      }
+      assert (action_order_some : action_order <> []).
+      { 
+        intros H_empty.
+        subst action_order.
+        generalize (@finite_surjective (spec_action tf_ctx) (spec_action_fin tf_ctx) cmd). intros H1.
+        rewrite H_empty in H1.
+        rewrite nth_error_nil in H1. inversion H1.
+      }
+      assert (action_order_has_cmd : In cmd action_order).
+      { 
+        subst action_order.
+        generalize (@finite_surjective (spec_action tf_ctx) (spec_action_fin tf_ctx) cmd). intros H1.
+        apply nth_error_In with (finite_index cmd). exact H1.
+      }
+
+      induction (action_order).
+      { destruct action_order_some. reflexivity. }
+      {
+        timeout 10 cbn -[some_rules UntypedLogs.log_empty].
+
+        destruct (eq_dec a cmd).
+        {
+          subst a. assert (H_not_in_l: ~ In cmd l). { inversion H0. timeout 10 sauto. }
+          
+          assert ((~ Common.scheduler_has_rule (fold_right (fun (t : some_fs_action) (acc : scheduler) => rule_cmd tf_ctx t |> acc) (done) l) (rule_cmd tf_ctx cmd))).
+          {
+            unfold not. unfold Common.scheduler_has_rule. intros H_in.
+            clear IHl. induction l.
+            { timeout 10 sauto. }
+            {
+              destruct (eq_dec a cmd) as [H_eq | H_neq].
+              { timeout 10 sauto. }
+              { 
+                timeout 10 cbn [fold_right Common.scheduler_has_rule] in H_in. 
+                destruct (eq_dec (rule_cmd tf_ctx a) (rule_cmd tf_ctx cmd)) as [H_eq2 | H_neq2].
+                apply cmd_rule_eq_dec_equal in H_eq2. subst a. contradiction.
+                apply IHl. timeout 10 sauto. timeout 10 sauto. timeout 10 sauto. timeout 10 sauto.
+                exact H_in.                
+              }
+            }
+          }
+
+          case_eq (@UntypedSemantics.interp_rule pos_t var_t fn_name_t EqDec_string (reg_t tf_ctx) ext_fn_t (@ContextEnv some_reg_t some_reg_t_finite) hw_reg_state sigma (@UntypedLogs.log_empty val (reg_t tf_ctx) (@ContextEnv some_reg_t some_reg_t_finite)) (some_rules (rule_cmd tf_ctx cmd))).
+          {
+            intros. rewrite (interp_scheduler_no_cmd hw_reg_state cmd). reflexivity. exact H. exact H1.
+          }
+          {
+            intros. rewrite (interp_scheduler_no_cmd hw_reg_state cmd). reflexivity. exact H. exact H1.
+          }
+        }
+        {
+          rewrite interp_rule_wrong_cmd.
+          {
+            inversion action_order_has_cmd. congruence.
+            inversion H0. subst l0 x.
+            destruct (eq_dec l []).
+            { subst l. contradiction. }
+            {
+              apply IHl.
+              timeout 10 sauto.
+              timeout 10 sauto.
+              timeout 10 sauto.
+            }
+          }
+          {
+            unfold not. intros. assert (encoded_cmd cmd = encoded_cmd a). { timeout 10 sauto. } apply encoded_cmd_inj' in H2. contradiction. timeout 10 sauto.
+          }
+        }
+      }
+    Qed. 
+    
+    Lemma interp_rule_right_cmd:
+      forall (hw_reg_state: hw_env_t) log cmd,
+      sigma (ext_in_cmd tf_ctx) val_true = encoded_cmd cmd ->
+      UntypedSemantics.interp_rule hw_reg_state sigma log (some_rules (rule_cmd tf_ctx cmd)) = 
+      UntypedSemantics.interp_rule hw_reg_state sigma log (_rule_cmd tf_ctx cmd).
+    Proof.
+      intros.
+      unfold some_rules.
+      unfold UntypedSemantics.interp_rule.
+      unfold UntypedSemantics.interp_action.
+      cbn -[_rule_cmd].
+
+      set (sigma_val := sigma (ext_in_cmd tf_ctx) (Bits [true])) in *.
+      assert (HSigmaValCmd: sigma_val = encoded_cmd cmd).
+      { unfold sigma_val. exact H. } rewrite HSigmaValCmd in *. clear sigma_val HSigmaValCmd. clear H.
+      cbn -[_rule_cmd].
+
+      (* Help out unpacking the relevant spec_action_index info from tf_ctx *)
+      unfold _fs_cmd_encoding, some_cmd_reg_size, spec_action_index, spec_action, spec_action_fin in *.
+      assert (@finite_index some_fs_action some_fs_action_fin cmd = @finite_index (spec_action tf_ctx) (spec_action_fin tf_ctx) cmd).
+      { unfold tf_ctx, tf_spec_action, tf_spec_action_fin in *. fold tf_ctx in *. reflexivity. } rewrite H in *; clear H.
+
+      (* Help out with the comparison *)
+      set (eq_true := BitsToLists.list_eqb _ _ _) in *.
+      assert (eq_true = true).
+      { unfold eq_true. apply BitsToLists.list_eqb_refl. intros. destruct a. timeout 10 sauto. timeout 10 sauto. } rewrite H in *; clear H. clear eq_true.
+
+      unfold opt_bind.
+      cbn.
+      reflexivity.
+    Qed.
+
+  End CmdGuard.
+
+  Section ActionInterpretation.
+
+    Lemma interp_act_read_state_vars {REnv : Env some_reg_t} : 
+      forall (hw_reg_state: hw_env_t) (Gamma: list (string * val)) sched_log action_log code state_list,
+      (* Precondition: Ensure all reads performed by the wrapper will succeed. *)
+      (forall (reg: some_reg_t), UntypedLogs.log_existsb sched_log reg UntypedLogs.is_write1 = false) ->
+
+      UntypedSemantics.interp_action hw_reg_state sigma Gamma sched_log action_log (_rule_read_state_vars_rec tf_ctx state_list code) =
+      
+      (* 1. Pre-calculate the values of all state registers that would be read. *)
+      let state_values := List.map (fun s =>
+        let v := match UntypedLogs.latest_write0 (UntypedLogs.log_app action_log sched_log) (tf_reg tf_ctx s) with
+                | Some v => v
+                | None => hw_reg_state.[(tf_reg tf_ctx s)]
+                end
+        in (_reg_name tf_ctx s, v)
+      ) (List.rev state_list) in
+
+      (* 2. Pre-calculate the log entries that would be generated by these reads. *)
+      let read_logs := List.fold_left (fun (acc_log: UntypedLogs._ULog) s =>
+        UntypedLogs.log_cons (tf_reg tf_ctx s) (UntypedLogs.LE Logs.LogRead P1 (Bits [])) acc_log
+      ) state_list action_log in
+
+      (* 3. The result is equivalent to interpreting [code] with the pre-calculated
+            context and log, then packaging the result. The final Gamma is unchanged
+            because UBind cleans up after itself. *)
+      match UntypedSemantics.interp_action hw_reg_state sigma (state_values ++ Gamma) sched_log read_logs code with
+      | Some (final_log, v, Gamma') => Some (final_log, v, skipn (List.length state_list) Gamma')
+      | None => None
+      end.
+    Proof.
+      intros.
+
+      generalize dependent Gamma.
+      generalize dependent action_log.
+      induction state_list.
+      {
+        intros. timeout 10 simpl.
+        case_eq (UntypedSemantics.interp_action hw_reg_state sigma Gamma sched_log action_log code).
+        - intros. destruct p as [ [final_log v] Gamma']. reflexivity.
+        - intros. reflexivity.
+      }
+      {
+        intros. timeout 10 simpl. unfold opt_bind.
+        rewrite H. timeout 10 simpl.
+
+        rewrite IHstate_list. clear IHstate_list.
+        timeout 10 simpl.
+
+        match goal with
+        | [ |- match ?E with _ => _ end = _ ] =>
+          remember E as LM
+        end.
+        match goal with
+        | [ |- _ = match ?E with _ => _ end ] =>
+          remember E as RM
+        end.
+        match goal with
+        | [ HeqLM : _ = match ?E with _ => _ end |- _] =>
+          remember E as LMM
+        end.
+        rewrite HeqLM. clear HeqLM.
+
+        assert (Heq: LMM = RM). 
+        {
+          rewrite HeqLMM. rewrite HeqRM.
+          clear HeqLMM. clear HeqRM.
+          f_equal.
+          {
+            unfold UntypedLogs.latest_write0.
+            rewrite map_app. timeout 10 simpl.
+            rewrite <- app_assoc. timeout 10 simpl.
+            
+            match goal with
+            | [ |- ?A ++ ?C = ?B ++ ?C ] =>
+              assert (A = B)
+            end.
+            {
+              f_equal. extensionality s. f_equal. 
+              set (lhs := UntypedLogs.log_find _ _ _).
+              set (rhs := UntypedLogs.log_find _ _ _).
+              assert (lhs = rhs) as H0.
+              {
+                subst lhs; subst rhs.
+                destruct (eq_dec (tf_reg tf_ctx s) (tf_reg tf_ctx a)).
+                {
+                  rewrite e. clear e.
+                  timeout 10 simpl.
+                  unfold UntypedLogs.log_find.
+                  unfold getenv. cbn.
+                  rewrite !cassoc_ccreate. 
+                  rewrite !cassoc_creplace_eq. cbn.
+                  reflexivity. 
+                } {
+                  timeout 10 simpl.
+                  unfold UntypedLogs.log_find.
+                  unfold getenv. cbn.
+                  rewrite !cassoc_ccreate. 
+                  rewrite !cassoc_creplace_neq_k.
+                  timeout 10 sauto.
+                  timeout 10 sauto.
+                }
+              } rewrite H0. reflexivity.
+            } rewrite H0. reflexivity. 
+          }
+        } 
+        
+        rewrite Heq. clear Heq. clear HeqLMM. clear HeqRM.
+
+        case_eq RM.
+        {
+          intros. destruct p as [p0 Gamma']. destruct p0 as [final_log v].
+          f_equal. destruct Gamma' as [| h t] eqn:E. 
+          { 
+            rewrite skipn_nil. reflexivity.
+          } {
+            f_equal. remember (Datatypes.length _) as len.
+            destruct len.
+            - rewrite skipn_O. rewrite skipn_O. reflexivity.
+            - rewrite skipn_cons. assert (tl (skipn len t) = skipn 1 (skipn len t)) as H_tl_is_skipn1.
+              {
+                destruct (skipn len t) eqn:E2.
+                { rewrite skipn_nil. reflexivity. }
+                { reflexivity. }
+              } rewrite H_tl_is_skipn1. clear H_tl_is_skipn1.
+              rewrite skipn_skipn. reflexivity.  
+          }
+        }
+        {
+          intros. reflexivity.
+        }
+      }
+    Qed. 
+
+    Lemma interp_act_write_state_vars {REnv : Env some_reg_t} : 
+      forall (hw_reg_state: hw_env_t) (Gamma: list (string * val)) sched_log action_log state_op,
+      (* Precondition: Ensure all writes performed by the wrapper will succeed. *)
+      (* (forall (reg: some_reg_t), UntypedLogs.log_existsb sched_log reg UntypedLogs.is_write0 = false) -> *)
+
+      (* (forall (reg: some_reg_t), let combined_log := (@ccreate some_reg_t (fun _ : some_reg_t => list (UntypedLogs.LogEntry val)) (@finite_elements some_reg_t some_reg_t_finite)
+              (fun (k : some_reg_t) (_ : @member some_reg_t k (@finite_elements some_reg_t some_reg_t_finite)) =>
+              @app (UntypedLogs.LogEntry val) (@getenv some_reg_t (@ContextEnv some_reg_t some_reg_t_finite) (fun _ : some_reg_t => list (UntypedLogs.LogEntry val)) action_log k)
+              (@getenv some_reg_t (@ContextEnv some_reg_t some_reg_t_finite) (fun _ : some_reg_t => list (UntypedLogs.LogEntry val)) sched_log k))) in
+          (@UntypedLogs.log_existsb val some_reg_t (@ContextEnv some_reg_t some_reg_t_finite) combined_log reg UntypedLogs.is_read1 = false
+          /\ @UntypedLogs.log_existsb val some_reg_t (@ContextEnv some_reg_t some_reg_t_finite) combined_log reg UntypedLogs.is_write1 = false
+          /\ @UntypedLogs.log_existsb val some_reg_t (@ContextEnv some_reg_t some_reg_t_finite) combined_log reg UntypedLogs.is_write0 = false)) -> *)
+
+      let written_vars := List.filter (fun s => if (tf_op_var_not_written_dec some_fs_states some_fs_states_fin some_fs_states_size s state_op) then false else true) some_fs_state_elements in
+
+      (* Precondition: Ensure all writes performed by the wrapper will succeed. *)
+      (* (forall (reg: some_reg_t), UntypedLogs.log_existsb sched_log reg UntypedLogs.is_write0 = false) -> *)
+
+      (forall s, let reg := tf_reg tf_ctx s in let combined_log := (@ccreate some_reg_t (fun _ : some_reg_t => list (UntypedLogs.LogEntry val)) (@finite_elements some_reg_t some_reg_t_finite)
+              (fun (k : some_reg_t) (_ : @member some_reg_t k (@finite_elements some_reg_t some_reg_t_finite)) =>
+              @app (UntypedLogs.LogEntry val) (@getenv some_reg_t (@ContextEnv some_reg_t some_reg_t_finite) (fun _ : some_reg_t => list (UntypedLogs.LogEntry val)) action_log k)
+              (@getenv some_reg_t (@ContextEnv some_reg_t some_reg_t_finite) (fun _ : some_reg_t => list (UntypedLogs.LogEntry val)) sched_log k))) in
+          In s written_vars -> @UntypedLogs.log_existsb val some_reg_t (@ContextEnv some_reg_t some_reg_t_finite) combined_log reg UntypedLogs.is_write1 = false) ->
+
+      (* Precondition: Ensure all written vars have values in Gamma *)
+      (forall s, In s written_vars -> exists v, BitsToLists.list_assoc Gamma (_reg_name tf_ctx s) = Some v) ->
+
+      let val_for_state := fun s => match BitsToLists.list_assoc Gamma (_reg_name tf_ctx s) with
+      | Some v => v
+      | None => hw_reg_state.[tf_reg tf_ctx s]
+      end
+      in
+
+      let write_logs := List.fold_left (fun (acc_log: UntypedLogs._ULog) s =>
+        UntypedLogs.log_cons (tf_reg tf_ctx s) (UntypedLogs.LE Logs.LogWrite P1 (val_for_state s)) acc_log
+      ) written_vars action_log in 
+
+      UntypedSemantics.interp_action hw_reg_state sigma Gamma sched_log action_log (_rule_write_state_vars tf_ctx state_op {{ pass }}) =
+      Some (write_logs, Bits [], Gamma).
+    Proof.
+      intros.
+      
+      generalize dependent H.
+      generalize dependent H0.
+
+      unfold _rule_write_state_vars, spec_all_states, some_fs_state_elements, spec_states, spec_states_fin, tf_spec_states, tf_spec_states_fin in *.
+      timeout 10 simpl. 
+
+      generalize finite_injective.
+      generalize finite_surjective.
+      intros H_inj H_surj.
+
+      subst written_vars.
+      subst val_for_state.
+      subst write_logs.
+      set (StateList := finite_elements). 
+      set (RegList := finite_elements).
+
+      assert (NoDup StateList) as H_nodup.
+      { apply NoDup_map_inv with (f:=finite_index). apply finite_injective. }
+
+      generalize dependent action_log.
+      induction StateList; intros.
+      {
+        timeout 10 simpl. 
+        assert ((vect_to_list Ob) = []). { timeout 10 sauto. } rewrite H1.
+        timeout 10 sauto.
+      }
+      {
+        timeout 10 simpl.
+        destruct (tf_op_var_not_written_dec some_fs_states some_fs_states_fin some_fs_states_size a state_op).
+        {
+          apply IHStateList. inversion H_nodup. exact H4.
+          intros. apply H0. timeout 10 sauto. intros. apply H. timeout 10 sauto.
+        }
+        {
+          timeout 10 simpl.
+
+          assert (exists v, BitsToLists.list_assoc Gamma (_reg_name tf_ctx a) = Some v) as [v H1].
+          { apply H0. timeout 10 sauto. } rewrite H1 in *. clear H1. timeout 10 simpl.
+          set (any_write1s := UntypedLogs.log_existsb _ _ _).
+          assert (any_write1s = false). { 
+            apply (H a). rewrite filter_In. split.
+            - apply in_eq. 
+              (* generalize (@finite_surjective some_fs_states some_fs_states_fin a). intros Hxx. apply nth_error_In with (finite_index a). exact Hxx. *)
+            - timeout 10 sauto.
+          }
+          rewrite H1. clear H1 any_write1s.
+          timeout 10 simpl.
+
+          rewrite IHStateList.
+          {
+            timeout 10 sauto.
+          } {
+            inversion H_nodup. exact H4.
+          } {
+            intros. apply H0. timeout 10 sauto.
+          } {
+            clear IHStateList.
+            intros.
+            assert (~ In a StateList) as H_not_in.
+            { inversion H_nodup. timeout 10 sauto. }
+
+            destruct (eq_dec s a).
+            { subst s. unfold not in H_not_in. apply filter_In in H1. timeout 10 sauto. }
+            {
+              assert (~ tf_op_var_not_written some_fs_states some_fs_states_fin some_fs_states_size s state_op). {
+                contradict H1. rewrite filter_In. timeout 10 sauto.
+              }
+              assert (In s (filter (fun s : some_fs_states => if tf_op_var_not_written_dec some_fs_states some_fs_states_fin some_fs_states_size s state_op then false else true) (a :: StateList))).
+              {
+                apply filter_In. split.
+                - apply filter_In in H1. destruct H1. timeout 10 sauto.
+                - timeout 10 sauto.
+              }
+              specialize (H s H3).
+              unfold UntypedLogs.log_existsb in *. unfold getenv in *. cbn -[_reg_name] in *. rewrite !cassoc_ccreate in *.
+              rewrite !cassoc_creplace_neq_k. timeout 10 sauto. timeout 10 sauto.
+            }
+          }
+        }
+      }
+    Qed.
+
+  End ActionInterpretation.
+
+  (* Prove next HW cycle = next Spec cycle *)
+    Definition _ur (x: some_reg_t) := val_of_value (some_r x).
+    Definition initial_hw_state := 
+        ContextEnv.(create) _ur.
+
+    Definition next_hw_cycle (hw_reg_state: env_t ContextEnv (fun _ : some_reg_t => val)) := 
+    UntypedSemantics.interp_cycle some_rules hw_reg_state sigma some_system_schedule.
+
+    (* TODO: Update once we have operation lists as input *)
+    Definition some_fs_step :=  tf_op_step_commit some_fs_states _ some_fs_states_size.
+    Definition some_fs_op_step_writes :=  tf_op_step_writes some_fs_states _ some_fs_states_size.
+
+    Definition StateR (hw_reg_state: env_t ContextEnv (fun _ : some_reg_t => val)) (fs_state: ContextEnv.(env_t) some_fs_states_t) :=
+        forall x, hw_reg_state.[tf_reg tf_ctx x] = val_of_value (fs_state.[x]).
+    
+    Theorem InitState_correct :
+        StateR initial_hw_state (ContextEnv.(create) some_fs_states_init).
+    Proof.
+        unfold initial_hw_state. intros x.
+        rewrite getenv_create. rewrite getenv_create. (* hammer. *)  hauto lq: on.
+    Qed.
+
+    Lemma latest_write_eq_some_fs_op_step_writes:
+      forall hw_reg_state fs_state cmd state_var,
+      sigma (ext_in_cmd tf_ctx) val_true = encoded_cmd cmd ->
+      StateR hw_reg_state fs_state ->
+      UntypedLogs.latest_write (UntypedSemantics.interp_scheduler some_rules hw_reg_state sigma some_system_schedule) (tf_reg tf_ctx state_var) 
+      = match (some_fs_op_step_writes fs_state state_var (some_fs_action_ops cmd)) with
+        | Some k => Some (val_of_value k)
+        | None => None
+      end.
+    Proof.
+        intros hw_reg_state fs_state cmd state_var H_sigma_eq_cmd H_state.
+        unfold StateR in H_state.
+
+        (* assert (H_hwstate_is_bits: forall (s: some_fs_states), exists x, hw_reg_state.[tf_reg tf_ctx s] = Bits x).
+        { 
+          unfold StateR in H_state. unfold some_fs_states_t in *. unfold tf_states_type in *.
+          intros. rewrite H_state. unfold val_of_value. timeout 10 eauto.
+        } *)
+
+        rewrite (interp_scheduler_only_cmd hw_reg_state cmd).
+        { unfold UntypedSemantics.interp_scheduler, UntypedSemantics.interp_scheduler'.
+          rewrite (interp_rule_right_cmd hw_reg_state).
+          { 
+            unfold _rule_cmd, UntypedSemantics.interp_rule.
+            unfold UntypedLogs.latest_write, UntypedLogs.log_find.
+
+            rewrite (@interp_act_read_state_vars ContextEnv).
+            {
+              simpl. unfold _rule_aux, spec_all_states. cbn -[_reg_name].  
+              destruct (some_fs_action_ops cmd) eqn:H_ops.
+              { (* nop *)
+                cbn -[_reg_name]. 
+                
+                rewrite (@interp_act_write_state_vars ContextEnv).
+                {
+                  rewrite filter_written_vars_nop.
+                  cbn -[_reg_name]. rewrite !Common.getenv_ccreate.
+                  rewrite app_nil_r. 
+                  set (RegList := finite_elements).
+                  set (StateList := finite_elements).
+                  
+                  cbn -[_reg_name].
+                  rewrite SemanticProperties.find_none_notb. reflexivity.
+                  intros. unfold UntypedLogs.log_latest_write_fn.
+                  destruct a. destruct kind. reflexivity.
+                  exfalso. contradict H. subst RegList. unfold getenv; cbn -[_reg_name].
+                  
+                  rewrite <- fold_left_rev_right.
+                  induction (rev StateList).
+                  { 
+                    cbn -[_reg_name].  rewrite cassoc_ccreate. timeout 10 sauto.
+                  }
+                  {
+                    cbn -[_reg_name].  destruct ( eq_dec (tf_reg tf_ctx a) (tf_reg tf_ctx state_var) ).
+                    { rewrite e. clear e. rewrite cassoc_creplace_eq. cbn -[_reg_name].  timeout 10 sauto. }
+                    { rewrite cassoc_creplace_neq_k. timeout 10 sauto. timeout 10 sauto. } 
+                  }
+                }
+                {
+                  intros. subst combined_log. unfold UntypedLogs.log_existsb, getenv. timeout 10 cbn -[_reg_name]. rewrite !cassoc_ccreate.
+                  rewrite !app_nil_r. 
+                  set (RegList := finite_elements).
+                  set (StateList := finite_elements).
+
+                  rewrite <- fold_left_rev_right.
+
+                  induction (rev StateList).
+                  { timeout 10 simpl. rewrite !cassoc_ccreate. timeout 10 sauto. }
+                  {
+                    timeout 10 simpl.  destruct ( eq_dec (tf_reg tf_ctx a) reg ).
+                    { rewrite e. clear e. rewrite cassoc_creplace_eq. cbn -[_reg_name]. apply IHl. }
+                    { rewrite cassoc_creplace_neq_k. timeout 10 sauto. timeout 10 sauto. } 
+                  }                
+                }
+                {
+                  intros. econstructor. rewrite filter_written_vars_nop in *. inversion H. Unshelve. timeout 10 sauto.         
+                }
+              }
+              { (* neg *)
+              
+                cbn -[_reg_name]. unfold opt_bind.
+                rewrite app_nil_r.
+              
+                set (read_val := BitsToLists.list_assoc _ _). assert (H_read_val: read_val = Some (hw_reg_state.[tf_reg tf_ctx x])).
+                {
+                  subst read_val. set (RegList := finite_elements).  set (StateList := finite_elements).
+
+                  assert (In x (rev StateList)) as H_in.
+                  { 
+                    subst StateList. generalize (@finite_surjective some_fs_states some_fs_states_fin x). intros H1. rewrite <- in_rev.
+                    apply nth_error_In with (finite_index x). exact H1.
+                  }
+                  assert (NoDup (rev StateList)) as H_nodup.
+                  {
+                    subst StateList. apply NoDup_rev. apply NoDup_map_inv with (f:=finite_index).
+                    apply finite_injective.
+                  }
+
+                  unfold UntypedLogs.latest_write0. unfold UntypedLogs.log_find. unfold getenv; cbn -[_reg_name].
+                  (* Set Printing All.                   *)
+                  set (f_nil := (fun _ _ => _)).
+                  assert (f_nil = (fun _ _ => [])).
+                  {
+                    subst f_nil. extensionality k. extensionality m.
+                    rewrite !cassoc_ccreate. timeout 10 sauto.
+                  } rewrite H. clear H f_nil.
+
+                  set (f_access := (fun _ => _)).
+                  assert (f_access = (fun s => (_reg_name tf_ctx s, hw_reg_state.[tf_reg tf_ctx s]))).
+                  {
+                    subst f_access. extensionality s.
+                    rewrite !cassoc_ccreate. timeout 10 sauto.
+                  } rewrite H. clear H f_access.
+
+                  induction (rev StateList).
+                  { timeout 10 sauto. }
+
+                  destruct (eq_dec a x).
+                  { rewrite e. subst RegList StateList. timeout 10 cbn -[_reg_name]. destruct string_rec. { reflexivity. } contradict n. timeout 10 sauto. }
+
+                  timeout 10 cbn -[_reg_name]. destruct string_rec. {
+                    contradict e. unfold not. intros. apply reg_name_injective in H. timeout 10 sauto.
+                  }
+
+                  apply in_inv in H_in. destruct H_in. timeout 10 sauto.
+                  inversion H_nodup. apply IHl. timeout 10 sauto. timeout 10 sauto.
+                } rewrite H_read_val. clear H_read_val read_val.
+
+                unfold UntypedSemantics.usigma1. 
+                rewrite H_state. cbn -[_reg_name]. 
+
+                rewrite (@interp_act_write_state_vars ContextEnv).
+                {
+                  rewrite filter_written_vars_neg in *.
+                  rewrite !Common.getenv_ccreate.
+                  rewrite <- !fold_left_rev_right.
+                  rewrite !app_nil_r.
+
+                  set (RegList := finite_elements).
+                  set (StateList := finite_elements).
+                  
+                  unfold getenv; cbn -[_reg_name].  unfold putenv; cbn -[_reg_name].  
+                  destruct (eq_dec x state_var).
+                  { (* The var we are interested in is the one we just negated, we should get Some new value *)
+                    rewrite e. clear e.
+                    rewrite cassoc_creplace_eq. cbn -[_reg_name].
+                    destruct string_rec. {
+                      unfold when_vars_match.
+                      destruct (@eq_dec some_fs_states (@EqDec_FiniteType some_fs_states some_fs_states_fin) state_var state_var).
+                      { 
+                        rewrite e0. f_equal. f_equal. 
+                        
+                        unfold Bits.neg, Bits.map.
+                        rewrite vect_to_list_map.
+                        reflexivity.
+                      } contradict n. timeout 10 sauto.
+                    } contradict n. timeout 10 sauto.
+                  } { (* The var we are interested in is unchanged, we should get None *)
+                    rewrite cassoc_creplace_neq_k.
+                    {
+                      unfold when_vars_match.
+                      destruct (@eq_dec some_fs_states (@EqDec_FiniteType some_fs_states some_fs_states_fin) x state_var).
+                      { contradict n. timeout 10 sauto. }
+
+                      cbn -[_reg_name].
+                      rewrite SemanticProperties.find_none_notb. reflexivity.
+                      intros. unfold UntypedLogs.log_latest_write_fn.
+                      destruct a. destruct kind. reflexivity.
+                      exfalso. contradict H. subst RegList. unfold getenv; cbn -[_reg_name].
+                      
+                      induction (rev StateList).
+                      { 
+                        cbn -[_reg_name].  rewrite cassoc_ccreate. timeout 10 sauto.
+                      }
+                      {
+                        cbn -[_reg_name].  destruct ( eq_dec (tf_reg tf_ctx a) (tf_reg tf_ctx state_var) ).
+                        { rewrite e. clear e. rewrite cassoc_creplace_eq. cbn -[_reg_name].  timeout 10 sauto. }
+                        { rewrite cassoc_creplace_neq_k. timeout 10 sauto. timeout 10 sauto. } 
+                      }
+                      
+                    } timeout 10 sauto.
+                  }
+                }
+                {
+                  intros. subst combined_log. unfold UntypedLogs.log_existsb, getenv. timeout 10 cbn -[_reg_name]. rewrite !cassoc_ccreate.
+                  rewrite !app_nil_r. 
+                  set (RegList := finite_elements).
+                  set (StateList := finite_elements).
+
+                  rewrite <- fold_left_rev_right.
+
+                  induction (rev StateList).
+                  { timeout 10 simpl. rewrite !cassoc_ccreate. timeout 10 sauto. }
+                  {
+                    timeout 10 simpl.  destruct ( eq_dec (tf_reg tf_ctx a) reg ).
+                    { rewrite e. clear e. rewrite cassoc_creplace_eq. cbn -[_reg_name]. apply IHl. }
+                    { rewrite cassoc_creplace_neq_k. timeout 10 sauto. timeout 10 sauto. } 
+                  }                
+                }
+                {
+                  intros. econstructor. rewrite filter_written_vars_neg in *. assert (s = x) by (timeout 10 sauto). subst s. timeout 10 sauto.         
+                }
+              }
+            }
+            {
+              unfold UntypedLogs.log_existsb. intros.
+              unfold existsb, getenv. cbn -[_reg_name].  
+              rewrite cassoc_ccreate.
+              timeout 10 sauto.
+            }
+          } exact H_sigma_eq_cmd.
+        } exact H_sigma_eq_cmd.
+    Qed.
+    
+    Theorem NextState_correct:
+        forall cmd fs_state hw_reg_state,
+        sigma (ext_in_cmd tf_ctx) val_true = encoded_cmd cmd ->
+        StateR hw_reg_state fs_state ->
+        StateR (next_hw_cycle hw_reg_state) (some_fs_step fs_state (some_fs_action_ops cmd)).
+    Proof.
+        intros cmd fs_state hw_reg_state H_sigma_eq_cmd H_state.
+
+        (* We consider each state var individually *)
+        intros state_var.
+
+        (* Create next state definitions & specialize state equivalence to the vars we consider *)
+        set (some_fs_step fs_state (some_fs_action_ops cmd)) as fs_state'.
+        unfold next_hw_cycle, StateR in *.
+        unfold some_reg_t in *.
+
+        (* Compute what the next functional state will be, then use the hypothesis to relate it to the previous hardware state *)
+        unfold some_fs_step, tf_op_step_commit, tf_op_step_writes in fs_state'.
+        destruct some_fs_action_ops eqn:H_ops.
+        { (* nop *)
+          subst fs_state'; rewrite getenv_create.
+          rewrite <- H_state.
+
+          unfold UntypedSemantics.interp_cycle, UntypedLogs.commit_update.
+          rewrite getenv_create.
+
+          rewrite (latest_write_eq_some_fs_op_step_writes hw_reg_state fs_state cmd).
+          { rewrite H_ops. cbn. reflexivity. }
+          { exact H_sigma_eq_cmd. }
+          { exact H_state. }
+        }
+        { (* neg *)
+          subst fs_state'; rewrite getenv_create.
+
+          unfold UntypedSemantics.interp_cycle, UntypedLogs.commit_update.
+          rewrite getenv_create.
+
+          rewrite (latest_write_eq_some_fs_op_step_writes hw_reg_state fs_state cmd).
+          { 
+            rewrite H_ops. cbn -[val_of_value]. 
+            unfold when_vars_match.
+            destruct (eq_dec x state_var).
+            {
+              rewrite H_state. subst x. reflexivity.
+            } {
+              rewrite H_state. reflexivity.
+            }
+          }
+          { exact H_sigma_eq_cmd. }
+          { exact H_state. }
+        }
+    Qed.
+
+End CompositionalCorrectness.
