coq/v2_2/Syntax.v
@@ -1,0 +1,24 @@
+Require Import Koika.Frontend.
+Require Import Koika.Std.
+Require Import Koika.Utils.Common.
+Require Import Koika.Utils.Environments.
+
+Require Import Hammer.Plugin.Hammer.
+Set Hammer GSMode 63.
+
+Section TrustformerSyntax.
+
+    (* Given some variables, inputs and outputs we define our syntax *)
+    Context (states_var: Type).
+    Context (inputs_var: Type).
+    Context (outputs_var: Type).
+
+    (* Atomic operations on variables *)
+    Inductive tf_ops :=
+        | tf_nop (* No operation *)
+        | tf_neg (x : states_var) (* Negate a variable *)
+        | tf_input (x : states_var) (y : inputs_var) (* Read input into variable *)
+        | tf_output (x : states_var) (y : outputs_var) (* Write variable to output *)
+        . 
+
+End TrustformerSyntax.
