coq/v2_2/Synthesis.v
@@ -1,0 +1,415 @@
+Require Import Koika.Frontend.
+Require Import Koika.Std.
+Require Import Koika.Utils.Common.
+Require Import Koika.Utils.Environments.
+Require Koika.Properties.SemanticProperties.
+Require Koika.KoikaForm.Untyped.UntypedSemantics.
+Require Import Koika.KoikaForm.SimpleVal.
+
+Require Import Trustformer.v2_2.Syntax.
+Require Import Trustformer.v2_2.Semantics.
+Require Import Trustformer.v2_2.Utils.
+Require Trustformer.v2_2.Properties.Common.
+From Koika.Utils Require Import Tactics.
+
+Require Import Streams.
+Require Import Coq.Lists.List.
+Require Import Coq.Strings.String.
+Require Import Coq.Logic.Eqdep_dec.
+Require Import Coq.Init.Tactics.
+Require Import Coq.Setoids.Setoid.
+
+Require Import Hammer.Plugin.Hammer.
+Set Hammer ATPLimit 5.
+Set Hammer GSMode 63.
+
+Record TFSynthContext := {
+  tf_spec_states : Type;
+  tf_spec_states_fin : FiniteType tf_spec_states;
+  tf_spec_states_names : Show tf_spec_states;
+  tf_spec_states_size : tf_spec_states -> nat;
+  tf_spec_states_init : forall x: tf_spec_states, tf_states_type tf_spec_states tf_spec_states_size x;
+
+  tf_spec_inputs : Type;
+  tf_spec_inputs_fin : FiniteType tf_spec_inputs;
+  tf_spec_inputs_names : Show tf_spec_inputs;
+  tf_spec_inputs_size : tf_spec_inputs -> nat;
+
+  tf_spec_outputs : Type;
+  tf_spec_outputs_fin : FiniteType tf_spec_outputs;
+  tf_spec_outputs_names : Show tf_spec_outputs;
+  tf_spec_outputs_size : tf_spec_outputs -> nat;
+
+  tf_spec_action : Type;
+  tf_spec_action_fin : FiniteType tf_spec_action;
+  tf_spec_action_names : Show tf_spec_action;
+  tf_spec_action_ops : tf_spec_action -> tf_ops tf_spec_states tf_spec_inputs tf_spec_outputs (* TODO: more than just a single op *)
+}.
+
+Ltac unfold_tfctx := repeat (
+  unfold tf_spec_states in * || unfold tf_spec_states_fin in * || unfold tf_spec_states_names in * || unfold tf_spec_states_size in * 
+  || unfold tf_spec_states_init in * 
+  
+  || unfold tf_spec_inputs in * || unfold tf_spec_inputs_fin in * || unfold tf_spec_inputs_names in * || unfold tf_spec_inputs_size in * 
+  
+  || unfold tf_spec_outputs in * || unfold tf_spec_outputs_fin in * || unfold tf_spec_outputs_names in * || unfold tf_spec_outputs_size in * 
+  
+  || unfold tf_spec_action in * || unfold tf_spec_action_fin in * || unfold tf_spec_action_names in * 
+  
+  || unfold tf_spec_action_ops in *).
+
+Section TrustformerSynthesis.
+
+    Context (tf_synth_ctx: TFSynthContext).
+
+    (* ====== Abbreviations ====== *)
+
+    Definition spec_states := tf_spec_states tf_synth_ctx.
+    Definition spec_states_fin : FiniteType spec_states := tf_spec_states_fin tf_synth_ctx.
+    Definition spec_states_size := tf_spec_states_size tf_synth_ctx.
+    Definition spec_states_t := tf_states_type spec_states spec_states_size.
+    Definition spec_states_init := tf_spec_states_init tf_synth_ctx.
+    Definition spec_all_states := @finite_elements spec_states spec_states_fin.
+    Definition spec_state_index := @finite_index spec_states spec_states_fin.
+    Definition spec_state_num := List.length spec_all_states.
+
+    Definition spec_inputs := tf_spec_inputs tf_synth_ctx.
+    Definition spec_inputs_fin : FiniteType spec_inputs := tf_spec_inputs_fin tf_synth_ctx.
+    Definition spec_inputs_size := tf_spec_inputs_size tf_synth_ctx.
+    Definition spec_inputs_t := tf_inputs_type spec_inputs spec_inputs_size.
+    Definition spec_all_inputs := @finite_elements spec_inputs spec_inputs_fin.
+    Definition spec_input_index := @finite_index spec_inputs spec_inputs_fin.
+    Definition spec_input_num := List.length spec_all_inputs.
+
+    Definition spec_outputs := tf_spec_outputs tf_synth_ctx.
+    Definition spec_outputs_fin : FiniteType spec_outputs := tf_spec_outputs_fin tf_synth_ctx.
+    Definition spec_outputs_size := tf_spec_outputs_size tf_synth_ctx.
+    Definition spec_outputs_t := tf_outputs_type spec_outputs spec_outputs_size.
+    Definition spec_all_outputs := @finite_elements spec_outputs spec_outputs_fin.
+    Definition spec_output_index := @finite_index spec_outputs spec_outputs_fin.
+    Definition spec_output_num := List.length spec_all_outputs.
+
+    Definition spec_action := tf_spec_action tf_synth_ctx.
+    Definition spec_action_fin := tf_spec_action_fin tf_synth_ctx.
+    Definition spec_all_actions := @finite_elements spec_action spec_action_fin.
+    Definition spec_action_index := @finite_index spec_action spec_action_fin.
+    Definition spec_action_num := List.length spec_all_actions.
+
+    Definition spec_action_ops := tf_spec_action_ops tf_synth_ctx.
+
+
+    Instance show_spec_states : Show spec_states := tf_spec_states_names tf_synth_ctx.
+    Instance show_spec_inputs : Show spec_inputs := tf_spec_inputs_names tf_synth_ctx.
+    Instance show_spec_outputs : Show spec_outputs := tf_spec_outputs_names tf_synth_ctx.
+    Instance show_spec_action : Show spec_action := tf_spec_action_names tf_synth_ctx.
+
+   Ltac unfold_specs := repeat (
+      unfold spec_states in * || unfold spec_states_fin in * || unfold spec_states_size in * || unfold spec_states_t in *
+       || unfold spec_states_init in * || unfold spec_all_states in * || unfold spec_state_index in * || unfold spec_state_num in * 
+       
+       || unfold spec_inputs in * || unfold spec_inputs_fin in * || unfold spec_inputs_size in * || unfold spec_inputs_t in * 
+       || unfold spec_all_inputs in * || unfold spec_input_index in * || unfold spec_input_num in * 
+       
+       || unfold spec_outputs in * || unfold spec_outputs_fin in * || unfold spec_outputs_size in * || unfold spec_outputs_t in * 
+       || unfold spec_all_outputs in * || unfold spec_output_index in * || unfold spec_output_num in * 
+       
+       || unfold spec_action in * || unfold spec_action_fin in * || unfold spec_all_actions in * || unfold spec_action_index in * 
+       || unfold spec_action_num in * 
+       
+       || unfold spec_action_ops in *).
+    
+    Ltac unfold_specs_tfctx := unfold_specs ; unfold_tfctx.
+
+    Definition spec_var_not_written_dec := tf_op_var_not_written_dec spec_states spec_states_fin spec_inputs spec_outputs spec_states_size spec_inputs_size spec_outputs_size.
+    Definition spec_no_output_dec := tf_op_no_output_dec spec_states spec_states_fin spec_inputs spec_outputs spec_outputs_fin spec_states_size spec_inputs_size spec_outputs_size.
+
+    (* ====== Registers ====== *)
+
+    Inductive reg_t := 
+    | tf_reg (x : spec_states)
+    | tf_out (x : spec_outputs)
+    | tf_out_ack (x : spec_outputs)
+    .
+
+    Instance _reg_t_finite : FiniteType reg_t.
+    Proof.
+      econstructor.
+      instantiate (1 := fun x => 
+        match x with
+        |  tf_reg y => spec_state_index y
+        |  tf_out y => spec_state_num + spec_output_index y
+        |  tf_out_ack y => spec_state_num + spec_output_num + spec_output_index y
+        end).
+      instantiate (1 := 
+        map (fun x => tf_reg x) spec_all_states
+        ++ map (fun x => tf_out x) spec_all_outputs
+        ++ map (fun x => tf_out_ack x) spec_all_outputs).
+      {
+        intros. unfold_specs. destruct a. 
+        {
+          rewrite nth_error_app1. rewrite nth_error_map. rewrite (@finite_surjective spec_states spec_states_fin _). 
+          (* hammer. *) sfirstorder.
+          rewrite <- nth_error_Some. rewrite nth_error_map. rewrite (@finite_surjective spec_states spec_states_fin _).
+          (* hammer. *) sfirstorder.
+        }
+        {
+          rewrite nth_error_app2. rewrite nth_error_app1.
+          rewrite Nat.add_comm. rewrite map_length. rewrite Nat.add_sub.
+          rewrite nth_error_map. rewrite (@finite_surjective spec_outputs spec_outputs_fin _). 
+          (* hammer. *) sfirstorder.
+          rewrite !map_length. rewrite Nat.add_comm. rewrite Nat.add_sub. 
+          generalize (@finite_surjective spec_outputs spec_outputs_fin x). intros.
+          apply nth_error_Some.
+          (* hammer. *) scongruence use: @finite_surjective unfold: spec_outputs, tf_spec_outputs.
+          rewrite !map_length. 
+          (* hammer. *) sfirstorder.
+        }
+        {
+          rewrite nth_error_app2. rewrite nth_error_app2.
+          rewrite Nat.add_comm. rewrite Nat.add_comm. rewrite !map_length.
+          rewrite Nat.add_comm. rewrite Nat.add_assoc. rewrite Nat.add_comm. rewrite Nat.add_assoc.
+          rewrite Nat.add_sub. rewrite Nat.add_comm. rewrite Nat.add_sub.
+          rewrite nth_error_map. rewrite (@finite_surjective spec_outputs spec_outputs_fin _). 
+          (* hammer. *) sfirstorder.
+          rewrite !map_length. rewrite Nat.add_comm. rewrite Nat.add_comm. rewrite Nat.add_comm. rewrite Nat.add_assoc.
+          rewrite Nat.add_comm. rewrite Nat.add_assoc. rewrite Nat.add_sub. lia.
+          rewrite !map_length. lia.
+        }
+      }
+      {
+        rewrite map_app. rewrite !map_map. apply NoDup_app. 
+        assert ((fun x : spec_states => spec_state_index x) = spec_state_index) by reflexivity. rewrite H. clear H.
+        apply (@finite_injective spec_states spec_states_fin).
+        rewrite map_app. rewrite !map_map. apply NoDup_app.
+        {
+          apply FinFun.Injective_carac. apply Common.finite_elements_is_finfun_listing.
+          unfold FinFun.Injective. apply Common.finite_index_plus_constant_l_inj.
+        } {
+          apply FinFun.Injective_map_NoDup. unfold FinFun.Injective.
+          apply Common.finite_index_plus_constant_l_inj. apply Common.finite_elements_is_finfun_listing.
+        } {
+          intros. rewrite in_map_iff in H. rewrite in_map_iff in H0.
+          destruct H as [s1 [Hs1_in Hs1_eq]]. destruct H0 as [s2 [Hs2_in Hs2_eq]]. subst x.
+          rewrite <- Nat.add_assoc in Hs2_in. apply Nat.add_cancel_l in Hs2_in.
+          assert (spec_output_num > spec_output_index s1). {
+            apply Common.finite_index_in_range.
+          }
+          lia.
+        } {
+          intros. rewrite in_map_iff in H. rewrite in_map_iff in H0.
+          destruct H as [s1 [Hs1_in Hs1_eq]]. destruct H0 as [s2 [Hs2_in Hs2_eq]]. subst x.
+          destruct s2.
+          {
+            apply in_app_or in Hs2_eq. destruct Hs2_eq as [Hs2_eq | Hs2_eq].
+            apply in_map_iff in Hs2_eq. destruct Hs2_eq as [s2' [Hs2'_in Hs2'_eq]]. subst.
+            congruence.
+            apply in_map_iff in Hs2_eq. destruct Hs2_eq as [s2' [Hs2'_in Hs2'_eq]]. subst.
+            congruence.
+          } {
+            assert (spec_state_num > spec_state_index s1). {
+              apply Common.finite_index_in_range.
+            }
+            lia.
+          } {
+            assert (spec_state_num > spec_state_index s1). {
+              apply Common.finite_index_in_range.
+            }
+            lia.
+          }
+        }
+      }
+    Defined.
+
+    Instance eq_dec_states : EqDec spec_states.
+    Proof.
+      pose spec_states_fin.  
+      apply EqDec_FiniteType.
+    Defined.
+
+    Instance eq_dec_outputs : EqDec spec_outputs.
+    Proof.
+      pose spec_outputs_fin.  
+      apply EqDec_FiniteType.
+    Defined.
+
+    Definition _reg_name (x: spec_states) : string :=
+      "tf_st_" ++ string_id_of_nat (spec_state_index x).
+
+    Definition _out_name (x: spec_outputs) : string :=
+      "tf_out_" ++ string_id_of_nat (spec_output_index x).
+
+    Instance reg_names : Show reg_t :=
+      { show := fun r => match r with
+          | tf_reg x => String.append "reg_" (show x)
+          | tf_out x => String.append "out_" (show x)
+          | tf_out_ack x => String.append "out_ack_" (show x)
+          end
+      }.
+
+    (* ====== Register Types ====== *)
+
+    Definition R (r: reg_t) :=
+    match r with
+    | tf_reg x => spec_states_t x
+    | tf_out x => spec_outputs_t x
+    | tf_out_ack x => bits_t 1
+    end.
+
+    Definition r (reg: reg_t) : R reg :=
+      match reg with
+      | tf_reg x => spec_states_init x
+      | tf_out x => Bits.zero
+      | tf_out_ack x => Bits.zero
+      end.
+
+    (* ====== External Functions ====== *)
+
+    Inductive ext_fn_t := 
+    | ext_in_cmd
+    | ext_input (x : spec_inputs)
+    | ext_output (x : spec_outputs)
+    .
+
+    Definition cmd_reg_size := @Common.finite_bits_needed spec_action spec_action_fin.
+
+    Definition Sigma (fn: ext_fn_t) : ExternalSignature :=
+      match fn with
+      | ext_in_cmd => {$ bits_t 1 ~> maybe (bits_t cmd_reg_size) $}
+      | ext_input x => {$ bits_t 1 ~> spec_inputs_t x $}
+      | ext_output x => {$ spec_outputs_t x ~> bits_t 1 $}
+      end.
+
+    Definition ext_fn_specs (fn : ext_fn_t) := 
+      match fn with
+      | ext_in_cmd => {| efr_name := "in_cmd"; 
+                        efr_internal := false |}
+      | ext_input x => {| efr_name := String.append "in_param_" (show x); 
+                          efr_internal := false |}
+      | ext_output x => {| efr_name := String.append "out_param_" (show x); 
+                           efr_internal := false |}
+      end.
+
+    Instance ext_fn_names : Show ext_fn_t :=
+      { show := fun r => match r with
+          | ext_in_cmd => "in_cmd"
+          | ext_input x => String.append "in_param_" (show x)
+          | ext_output x => String.append "out_param_" (show x)
+          end
+      }.
+    
+    (* ====== Rules ====== *)
+
+    Inductive rule_name_t :=
+    | rule_cmd (cmd: spec_action)
+    | rule_out (out: spec_outputs)
+    .
+
+    Instance rule_names : Show rule_name_t :=
+      { show := fun r => match r with
+          | rule_cmd cmd => String.append "rule_cmd_" (show cmd)
+          | rule_out out => String.append "rule_out_" (show out)
+          end
+      }.
+
+    Definition system_schedule_outputs : scheduler := 
+      List.fold_right (fun t acc => rule_out t |> acc) Done spec_all_outputs.
+
+    Definition system_schedule_actions : scheduler  :=
+      List.fold_right (fun t acc => rule_cmd t |> acc) system_schedule_outputs spec_all_actions.
+
+    Definition system_schedule := system_schedule_actions.
+    
+    Definition op_to_uaction (op: tf_ops spec_states spec_inputs spec_outputs) (code: uaction reg_t ext_fn_t) : uaction reg_t ext_fn_t :=
+      match op with
+      | tf_nop _ _ _ => code 
+      | tf_neg _ _ _ x => UBind (_reg_name x) (UUnop (UBits1 UNot) (UVar (_reg_name x))) code
+      | tf_input _ _ _ x y => UBind (_reg_name x) (UExternalCall (ext_input y) {{Ob~1}}) code
+      | tf_output _ _ _ x y => UBind (_out_name y) (UVar (_reg_name x)) code
+      end.
+
+    Definition _rule_aux
+      (state_op: tf_ops spec_states spec_inputs spec_outputs)
+      (code: uaction reg_t ext_fn_t)
+      : uaction reg_t ext_fn_t :=
+        op_to_uaction state_op code.
+
+    (* Helper function that reads all state registers into variables *)
+    Fixpoint _rule_read_state_vars_rec (states_to_read : list (spec_states)) (code: uaction reg_t ext_fn_t): uaction reg_t ext_fn_t :=
+      match states_to_read with
+      | [] => code
+      | x :: rest =>
+        UBind (_reg_name x) 
+          {{ read1(tf_reg x) }} 
+          (_rule_read_state_vars_rec rest code)
+      end.
+
+    (* Helper function that writes back all modified state variables *)
+    Definition _rule_write_state_vars (op: tf_ops spec_states spec_inputs spec_outputs) (code: uaction reg_t ext_fn_t) : uaction reg_t ext_fn_t  := 
+      List.fold_right (fun x acc => 
+        if spec_var_not_written_dec x op then
+          acc
+        else
+          USeq {{ write1(tf_reg x, `UVar (_reg_name x)`) }} acc
+      ) code spec_all_states.
+    
+    (* Helper function that writes back all modified output variables *)
+    Definition _rule_write_output_vars (op: tf_ops spec_states spec_inputs spec_outputs) (code: uaction reg_t ext_fn_t) : uaction reg_t ext_fn_t  := 
+      List.fold_right (fun x acc => 
+        if spec_no_output_dec x op then
+          acc
+        else
+          USeq {{ write0(tf_out x, `UVar (_out_name x)`) }} acc
+      ) code spec_all_outputs.
+
+    Definition _rule_cmd cmd : uaction reg_t ext_fn_t :=
+      let state_ops := spec_action_ops cmd in
+      _rule_read_state_vars_rec spec_all_states (
+        _rule_aux state_ops (
+          _rule_write_state_vars state_ops (
+            _rule_write_output_vars state_ops
+              {{ pass }}))).
+
+    Definition rules :=
+        (fun rl =>  match rl with
+          | rule_cmd cmd => 
+            let cmd_enc := Bits.of_nat cmd_reg_size (spec_action_index cmd) in
+            {{
+                  guard(get(extcall ext_in_cmd(Ob~1), valid));
+                  guard(get(extcall ext_in_cmd(Ob~1), data) == #cmd_enc);
+                  `_rule_cmd cmd`
+            }}
+          | rule_out out =>
+            UWrite P1 (tf_out_ack out) (UExternalCall (ext_output out) ({{ read1(tf_out out) }} ))
+          end).
+
+End TrustformerSynthesis.
+
+(* 
+  We need to override the type checking tactic, since by default it expects rules to have no parameters.
+  Specifically, we need to match the three components of a rule (name, tf_ctx, param) and destruct the param
+  so that there are no opaque values for the type checker.
+*)
+
+Ltac _tc_rules R Sigma uactions :=
+    let rule_name_t := _arg_type uactions in
+    let res := constr:(fun r: rule_name_t =>
+                        ltac:(destruct r eqn:? ;
+                                lazymatch goal with
+                                | [ H: _ = ?r1 ?r2 ?r3 |- _ ] =>
+                                    destruct r3 eqn:?;
+                                    lazymatch goal with
+                                    | [ H: _ = ?rr2 |- _ ] =>
+                                        let ua := constr:(uactions rr2) in
+                                        let ua := (eval hnf in ua) in
+                                        (_tc_action R Sigma (@List.nil (var_t * type)) constr:(unit_t) ua)
+                                    end
+                                | [ H: _ = ?rr |- _ ] =>
+                                    let ua := constr:(uactions rr) in
+                                    let ua := (eval hnf in ua) in
+                                    _tc_action R Sigma (@List.nil (var_t * type)) constr:(unit_t) ua
+                                end)) in
+    exact res.
+
+Notation tc_rules R Sigma actions :=
+    (ltac:(_tc_rules R Sigma actions)) (only parsing).
+
